\begin{exercise}{1}
We wrote the Euler-Lagrange equation for the function $P(y) = \int_0^1 F(y, y') \, dx$ as 
	$$\frac{d}{dx} \, \bigg(\frac{\partial{F}}{\partial{y'}}y' - \frac{\partial{F}}{\partial{y}}\bigg) = 0.$$

\begin{enumerate}
	\item[a)]
		For $F = F(y, y')$, prove the following identity:
			$$\frac{d}{dx} \, \bigg(\frac{\partial{F}}{\partial{y'}} - F \bigg) = y' \bigg[\frac{d}{dx} \, \frac{\partial{F}}{\partial{y'}} - \frac{\partial{F}}{\partial{y}}\bigg].$$
	\item[b)]
		Use the identity to show that the Euler-Lagrange equation is equivalent to 
			$$\frac{\partial{F}}{\partial{y'}}y' - F = C.$$

\end{enumerate}

\textbf{Proof}

\begin{enumerate}
	\item[a)] To show part a, note the following:
		\begin{align*}
			\frac{d}{dx} \, \bigg(\frac{\partial{F}}{\partial{y'}}y' - F \bigg) &= \frac{d}{dx} \, \frac{\partial{F}}{\partial{y'}}y' - \, \frac{d}{dx}F \\
			&= \frac{d}{dx} \, \frac{\partial{F}}{\partial{y'}}y' - \frac{\partial{F}}{\partial{y}} \, \frac{dy}{dx} \\
			&= y' \bigg(\frac{d}{dx} \, \frac{\partial{F}}{\partial{y'}} - \frac{\partial{F}}{\partial{y}}\bigg).
		\end{align*}

	\item[b)] For part b, we have that 
		$$\frac{d}{dx} \, \bigg(\frac{\partial{F}}{\partial{y'}} - F \bigg) = y' \bigg[\frac{d}{dx} \, \frac{\partial{F}}{\partial{y'}} - \frac{\partial{F}}{\partial{y}}\bigg] = 0 = \frac{d}{dx} \, \bigg(\frac{\partial{F}}{\partial{y'}}y' - \frac{\partial{F}}{\partial{y}}\bigg).$$
		We can integrate the left side with respect to $x$, and we see that 
			$$\int \frac{d}{dx} \, \bigg(\frac{\partial{F}}{\partial{y'}} - F \bigg) \, dx = 0 \rightarrow \frac{\partial{F}}{\partial{y'}} - F = C.$$
		It follows then that solving the Euler-Lagrange equation is equivalent to solving for $ \frac{\partial{F}}{\partial{y'}} - F = C.$




\end{enumerate}